case_study/RiscvPmp/LoopVerificationBinary.v
@@ -67,11 +67,11 @@ Import RiscvPmpValidContracts.
 
 Import RiscvPmpSignature.
 Module Import RiscvPmpShallowExecutor :=
-  MakeShallowExecutor RiscvPmpBase RiscvPmpSignature RiscvPmpProgram RiscvPmpSpecification.
+  MakeShallowExecutor RiscvPmpBase RiscvPmpSignature RiscvPmpProgram DefaultFailLogic RiscvPmpSpecification.
 
-Module Import RiscvPmpShallowSoundness := MakeShallowSoundness RiscvPmpBase RiscvPmpSignature RiscvPmpProgram RiscvPmpSpecification RiscvPmpShallowExecutor RiscvPmpProgramLogic.
+Module Import RiscvPmpShallowSoundness := MakeShallowSoundness RiscvPmpBase RiscvPmpSignature RiscvPmpProgram DefaultFailLogic RiscvPmpSpecification RiscvPmpShallowExecutor RiscvPmpProgramLogic.
 
-Module Import RiscvPmpSymbolic := MakeSymbolicSoundness RiscvPmpBase RiscvPmpSignature RiscvPmpProgram RiscvPmpSpecification RiscvPmpShallowExecutor RiscvPmpExecutor.
+Module Import RiscvPmpSymbolic := MakeSymbolicSoundness RiscvPmpBase RiscvPmpSignature RiscvPmpProgram DefaultFailLogic RiscvPmpSpecification RiscvPmpShallowExecutor RiscvPmpExecutor.
 
 Section Loop.
   Context `{sg : sailGS2 Σ}.
