case_study/RiscvPmp/ModelBinary.v
@@ -82,12 +82,12 @@ Module RiscvPmpModel2.
   Import RiscvPmpSpecification.
   Import RiscvPmpProgram.
 
-  Module RiscvPmpProgramLogic <: ProgramLogicOn RiscvPmpBase RiscvPmpSignature RiscvPmpProgram RiscvPmpSpecification.
-    Include ProgramLogicOn RiscvPmpBase RiscvPmpSignature RiscvPmpProgram RiscvPmpSpecification.
+  Module RiscvPmpProgramLogic <: ProgramLogicOn RiscvPmpBase RiscvPmpSignature RiscvPmpProgram DefaultFailLogic RiscvPmpSpecification.
+    Include ProgramLogicOn RiscvPmpBase RiscvPmpSignature RiscvPmpProgram DefaultFailLogic RiscvPmpSpecification.
   End RiscvPmpProgramLogic.
   Include RiscvPmpProgramLogic.
 
-  Include IrisInstanceWithContracts2 RiscvPmpBase RiscvPmpSignature RiscvPmpProgram
+  Include IrisInstanceWithContracts2 RiscvPmpBase RiscvPmpSignature RiscvPmpProgram DefaultFailLogic
     RiscvPmpSemantics RiscvPmpSpecification RiscvPmpIrisBase2  RiscvPmpIrisAdeqParams2 RiscvPmpIrisInstance2.
 
   Section ForeignProofs.
