theories/Iris/BinaryInstance.v
@@ -65,10 +65,10 @@ Import env.notations.
 
 Set Implicit Arguments.
 
-Module Type IrisInstance2 (B : Base) (SIG : Signature B) (PROG : Program B)
+Module Type IrisInstance2 (B : Base) (SIG : Signature B) (PROG : Program B) (FL : FailLogic)
   (SEM : Semantics B PROG) (IB2 : IrisBase2 B PROG SEM) (IAP : IrisAdeqParameters2 B PROG SEM IB2 IB2 IB2) :=
-  IrisPredicates2 B SIG PROG SEM IB2 <+ IrisSignatureRules2 B SIG PROG SEM IB2
-    <+ IrisAdequacy2 B SIG PROG SEM IB2 IAP.
+  IrisPredicates2 B SIG PROG SEM IB2 <+ IrisSignatureRules2 B SIG PROG FL SEM IB2
+    <+ IrisAdequacy2 B SIG PROG FL SEM IB2 IAP.
 
 (*  * The following module defines the parts of the Iris model that must depend on the Specification, not just on the Signature. *)
 (*  * This is kept to a minimum (see comment for the IrisPredicates module). *)
@@ -77,12 +77,13 @@ Module IrisInstanceWithContracts2
   (Import B     : Base)
   (Import SIG   : Signature B)
   (Import PROG  : Program B)
+  (Import FL    : FailLogic)
   (Import SEM   : Semantics B PROG)
   (Import SPEC  : Specification B SIG PROG)
   (Import IB2   : IrisBase2 B PROG SEM)
   (Import IAP   : IrisAdeqParameters2 B PROG SEM IB2 IB2 IB2)
-  (Import II    : IrisInstance2 B SIG PROG SEM IB2 IAP)
-  (Import PLOG  : ProgramLogicOn B SIG PROG SPEC).
+  (Import II    : IrisInstance2 B SIG PROG FL SEM IB2 IAP)
+  (Import PLOG  : ProgramLogicOn B SIG PROG FL SPEC).
 
   Section WithSailGS.
   Import ProgramLogic.
@@ -198,6 +199,7 @@ Module IrisInstanceWithContracts2
     - by iApply iris_rule_stm_seq.
     - iApply iris_rule_stm_assertk.
       iIntros "H". by iApply "trips".
+      destruct fail_rule_pre; auto.
     - by iApply iris_rule_stm_fail.
     - by iApply iris_rule_stm_read_register.
     - by iApply iris_rule_stm_write_register.
